restructuring message formats, adding some reliability lemmas

scripts/DAP_Transaction.thy
@@ -20,10 +20,10 @@ inductive_set daptrans :: "event list set" where
 
   | DT2: "\<lbrakk> evs2 \<in> daptrans;
           Gets Server \<lbrace> Agent A, Number T \<rbrace> \<in> set evs2;
-          Nonce r \<notin> used evs2;
-          r' = Crypt (shrK A) (Nonce r);
-          h\<^sub>s = Hash \<lbrace> \<lbrace> Agent A, Number T \<rbrace>, r' \<rbrace> \<rbrakk>
-    \<Longrightarrow> Says Server A \<lbrace> \<lbrace> Agent A, Number T \<rbrace>, r', h\<^sub>s \<rbrace> # evs2 \<in> daptrans"
+          Nonce r \<notin> used evs2 \<rbrakk>
+    \<Longrightarrow> Says Server A \<lbrace> \<lbrace> Agent A, Number T \<rbrace>, 
+                        Crypt (shrK A) (Nonce r), 
+                        Hash \<lbrace> \<lbrace>Agent A, Number T\<rbrace>, Crypt (shrK A) (Nonce r) \<rbrace> \<rbrace> # evs2 \<in> daptrans"
 
   | DT3: "\<lbrakk> evs3 \<in> daptrans; legalUse (Smartphone A);
             Says A Server \<lbrace> Agent A, Number T \<rbrace> \<in> set evs3;
@@ -33,16 +33,15 @@ inductive_set daptrans :: "event list set" where
   | DT4: "\<lbrakk> evs4 \<in> daptrans;
             legalUse(Smartphone A); A \<noteq> Server;
             Gets_s (Smartphone A) \<lbrace> Transaction', r', h\<^sub>s \<rbrace> \<in> set evs4;
-            h\<^sub>u = Hash \<lbrace> Transaction', r' \<rbrace>;
-            h\<^sub>s == h\<^sub>u \<rbrakk> 
+            h\<^sub>s == Hash \<lbrace> Transaction', r' \<rbrace> \<rbrakk> 
     \<Longrightarrow> Outputs (Smartphone A) A Transaction' # evs4 \<in> daptrans"
 
   | DT5: "\<lbrakk> evs5 \<in> daptrans;
-            Says A Server Transaction \<in> set evs5;
-            Gets A \<lbrace> Transaction, r', h\<^sub>s \<rbrace> \<in> set evs5;
-            Inputs A (Smartphone A) \<lbrace> Transaction, r', h\<^sub>s \<rbrace> \<in> set evs5;
+            Says A Server \<lbrace> Agent A, Number T \<rbrace> \<in> set evs5;
+            Gets A \<lbrace> \<lbrace> Agent A, Number T \<rbrace>, r', h\<^sub>s \<rbrace> \<in> set evs5;
+            Inputs A (Smartphone A) \<lbrace> \<lbrace> Agent A, Number T \<rbrace>, r', h\<^sub>s \<rbrace> \<in> set evs5;
             Gets_a A Transaction' \<in> set evs5;
-            Transaction == Transaction' \<rbrakk>
+            Transaction' == \<lbrace> Agent A, Number T \<rbrace> \<rbrakk>
     \<Longrightarrow> Inputs A (Smartphone A) Confirmation # evs5 \<in> daptrans"
 
   | DT6: "\<lbrakk> evs6 \<in> daptrans; A \<noteq> Server;
@@ -69,7 +68,8 @@ inductive_set daptrans :: "event list set" where
             r_u == r' \<rbrakk>
     \<Longrightarrow> Says Server A Success # evs8 \<in> daptrans"
 
-  | Fake: "\<lbrakk> evsF \<in> daptrans; X \<in> synth(analz(knows Spy evsF)) \<rbrakk> \<Longrightarrow> Says Spy B X # evsF \<in> daptrans"
+  | Fake: "\<lbrakk> evsF \<in> daptrans; X \<in> synth(analz(knows Spy evsF)); illegalUse(Smartphone B) \<rbrakk> 
+    \<Longrightarrow> Says Spy B X # Inputs Spy (Smartphone B) X # evsF \<in> daptrans"
     
   | Rcpt: "\<lbrakk> evsR \<in> daptrans; Says A B X \<in> set evsR \<rbrakk> \<Longrightarrow> Gets B X # evsR \<in> daptrans"
 
@@ -79,8 +79,10 @@ inductive_set daptrans :: "event list set" where
   | Rcpt_a: "\<lbrakk> evsRa \<in> daptrans; Outputs (Smartphone A) B X \<in> set evsRa \<rbrakk>
     \<Longrightarrow> Gets_a B X # evsRa \<in> daptrans"
 
+declare Fake_parts_insert_in_Un  [dest]
+declare analz_into_parts [dest]
 
-
+(* TECHNICAL LEMMAS *)
 lemma Gets_imp_Says :
   "\<lbrakk> Gets B X \<in> set evs; evs \<in> daptrans \<rbrakk> \<Longrightarrow> \<exists> A. Says A B X \<in> set evs"
 apply (erule rev_mp, erule daptrans.induct)
@@ -105,6 +107,15 @@ lemma Says_Server_DT1_not_evs :
   "evs \<in> daptrans \<Longrightarrow> Says Server Server \<lbrace> Agent Server, Number T \<rbrace> \<notin> set evs"
 apply (erule daptrans.induct)
 apply (simp_all)
+done
+
+lemma Says_Server_message_form_DT2 :
+  "\<lbrakk> evs \<in> daptrans; Says Server A \<lbrace> Transaction, r', Checksum \<rbrace> \<in> set evs \<rbrakk>
+    \<Longrightarrow> (\<exists> T. Transaction = \<lbrace> Agent A, Number T \<rbrace>) \<and>
+        (\<exists> r. r' = Crypt (shrK A) (Nonce r)) \<and>
+        Checksum = Hash \<lbrace> Transaction, r' \<rbrace>"
+apply (erule rev_mp, erule daptrans.induct)
+apply (auto)
 done
 
 (* TODO: ask Claudia how did I manage to do this *)
@@ -136,19 +147,37 @@ apply (auto)
 done
 
 
-
 (* PROTOCOL TERMINATION *)
+lemma DT2_happens :
+  "\<exists> T r. \<exists>evs \<in> daptrans. 
+    Says Server A \<lbrace> \<lbrace> Agent A, Number T\<rbrace>,
+      Crypt (shrK A) (Nonce r),
+      Hash \<lbrace> \<lbrace>Agent A, Number T\<rbrace>, Crypt (shrK A) (Nonce r) \<rbrace> \<rbrace> \<in> set evs"
+apply (intro exI bexI)
+apply (rule_tac [2] daptrans.DT2)
+apply (rule_tac [2] daptrans.Rcpt)
+apply (rule_tac [2] daptrans.DT1)
+apply (rule_tac [2] daptrans.Nil)
+apply (simp_all)
+apply (possibility, auto)
+oops
+
 lemma DT3_happens:
   "\<exists> T r h. \<exists>evs \<in> daptrans. Inputs A (Smartphone A) \<lbrace> T, r, h \<rbrace> \<in> set evs"
 apply (intro exI bexI)
-apply (rule_tac [2] daptrans.Nil 
+apply (rule_tac [2] daptrans.DT3)
+apply (rule_tac [2] daptrans.Rcpt)
+apply (rule_tac [2] daptrans.DT2)
+apply (rule_tac [2] daptrans.Rcpt)
+apply (rule_tac [2] daptrans.DT1)
+apply (rule_tac [2] daptrans.Nil)
+apply (simp_all)
+(* apply (rule_tac [2] daptrans.Nil 
         [THEN daptrans.DT1, THEN daptrans.Rcpt,
         THEN daptrans.DT2, THEN daptrans.Rcpt,
-        THEN daptrans.DT3])
-apply (simp_all)
-apply (possibility)
-apply (auto)
-done
+        THEN daptrans.DT3]) *)
+apply (possibility, auto)
+oops
 
 lemma DT4_happens:
   "\<exists> T. \<exists>evs \<in> daptrans. Outputs (Smartphone A) A T \<in> set evs"
@@ -159,7 +188,7 @@ apply (rule_tac [2] daptrans.Nil
         THEN daptrans.DT3, THEN daptrans.Rcpt_s,
         THEN daptrans.DT4])
 apply (possibility, auto)
-done
+oops
 
 lemma DT5_happens:
   "\<exists> C. \<exists>evs \<in> daptrans. Inputs A (Smartphone A) C \<in> set evs"
@@ -171,7 +200,7 @@ apply (rule_tac [2] daptrans.Nil
         THEN daptrans.DT4, THEN daptrans.Rcpt_a,
         THEN daptrans.DT5])
 apply (possibility, auto)
-done
+oops
 
 lemma DT6_happens :
   "\<exists> r\<^sub>u. \<exists> evs \<in> daptrans. Outputs (Smartphone A) A r\<^sub>u \<in> set evs"
@@ -184,7 +213,7 @@ apply (rule_tac [2] daptrans.Nil
         THEN daptrans.DT5, THEN daptrans.Rcpt_s,
         THEN daptrans.DT6])
 apply (possibility, auto)
-done
+oops
 
 lemma DT7_happens :
   "\<exists> r\<^sub>u. \<exists> evs \<in> daptrans. Says A Server r\<^sub>u \<in> set evs"
@@ -200,7 +229,7 @@ apply (rule_tac [2] daptrans.Nil
 apply (simp_all)
 apply (possibility)
 apply (auto)
-done
+oops
 
 lemma Protocol_terminates :
   "\<exists>Success. \<exists>evs \<in> daptrans. Says Server A Success \<in> set evs"
